\chapter{Polynomials and Their Graphs}

Find the degree, leading term, leading coefficient, and constant term of the following polynomials.
\begin{multicols}{3}
\begin{enumerate}
\item $f(x) = -x^5 + \sqrt{7}x^3 - 2x^2$
\item $g(x) = 4x^2 - 16x^6 + 3x$
\item $h(x) = 1 + x^{11} - 4x^8$
\end{enumerate}	\setcounter{Review}{\value{enumi}}
\end{multicols}
\begin{multicols}{3}
\begin{enumerate}	\setcounter{enumi}{\value{Review}} 
\item $f(x) = -x^4+3x^2-2x+6$
\item $g(x) = 0.25x^5-0.1x^4+2x^2-6x$
\item $f(x) = -6x^3 + 2x^2 + 7x^4 - 1$
\end{enumerate}	\setcounter{Review}{\value{enumi}}
\end{multicols}
\begin{multicols}{3}
\begin{enumerate}	\setcounter{enumi}{\value{Review}} 
\item $g(x) = \frac{1}{3}x^3 - \frac{\pi}{8}x^2 + x\sqrt{2} - 3^4$
\item $h(x) = 7(x+1)^2(x-2)^3$
\item $j(x) = -\frac{1}{2}\left(3x+2\right)^2(x-1)^5$
\end{enumerate}		\setcounter{Review}{\value{enumi}}
\end{multicols}
\bigskip

Determine the end behavior of each.
\begin{multicols}{3}
\begin{enumerate}	\setcounter{enumi}{\value{Review}}
\item $f(x) = -x^5 + \sqrt{7}x^3 - 2x^2$
\item $g(x) = 4x^2 - 16x^6 + 3x$
\item $h(x) = 1 + x^{11} - 4x^8$
\end{enumerate}	\setcounter{Review}{\value{enumi}}
\end{multicols}
\begin{multicols}{3}
\begin{enumerate}	\setcounter{enumi}{\value{Review}} 
\item $f(x) = -x^4+3x^2-2x+6$
\item $g(x) = 0.25x^5-0.1x^4+2x^2-6x$
\item $f(x) = -6x^3 + 2x^2 + 7x^4 - 1$
\end{enumerate}	\setcounter{Review}{\value{enumi}}
\end{multicols}
\begin{multicols}{3}
\begin{enumerate}	\setcounter{enumi}{\value{Review}} 
\item $g(x) = \frac{1}{3}x^3 - \frac{\pi}{8}x^2 + x\sqrt{2} - 3^4$
\item $h(x) = 5(x+1)^2(x-2)^3$
\item $j(x) = -\frac{1}{2}\left(3x+2\right)^2(x-1)^5$
\end{enumerate}	\setcounter{Review}{\value{enumi}}
\end{multicols}
\bigskip

Find the zeros of each. Round to 2 decimal places when necessary.
\begin{multicols}{3}
\begin{enumerate}	\setcounter{enumi}{\value{Review}}
\item $f(x) = -x^5 + \sqrt{7}x^3 - 2x^2$
\item $g(x) = 4x^2 - 16x^6 + 3x$
\item $h(x) = 1 + x^{11} - 4x^8$
\end{enumerate}	\setcounter{Review}{\value{enumi}}
\end{multicols}
\begin{multicols}{3}
\begin{enumerate}	\setcounter{enumi}{\value{Review}} 
\item $f(x) = -x^4+3x^2-2x+6$
\item $g(x) = 0.25x^5-0.1x^4+2x^2-6x$
\item $f(x) = -6x^3 + 2x^2 + 7x^4 - 1$
\end{enumerate}	\setcounter{Review}{\value{enumi}}
\end{multicols}
\begin{multicols}{3}
\begin{enumerate}	\setcounter{enumi}{\value{Review}} 
\item $g(x) = \frac{1}{3}x^3 - \frac{\pi}{8}x^2 + x\sqrt{2} - 3^4$
\item $h(x) = 5(x+1)^2(x-2)^3$
\item $j(x) = -\frac{1}{2}\left(3x+2\right)^2(x-1)^5$
\end{enumerate}	\setcounter{Review}{\value{enumi}}
\end{multicols}

\newpage

\section{Answer Key}

\begin{enumerate}
	\item Degree = 5, Leading Term = $-x^5$, Leading Coefficient = $-1$, Constant = none (or 0)
	\item Degree = 6, Leading Term = $-16x^6$, Leading Coefficient = $-16$, Constant = none (or 0)
	\item Degree = 11, Leading Term = $x^{11}$, Leading Coefficient = 1, Constant = 1
	\item Degree = 4, Leading Term = $-x^4$, Leading Coefficient = $-1$, Constant = 6
	\item Degree = 5, Leading Term = $0.25x^5$, Leading Coefficient = $0.25$, Constant = none (or 0)
	\item Degree = 3, Leading Term = $-6x^3$, Leading Coefficient = $-6$, Constant = $-1$
	\item Degree = 3, Leading Term = $\frac{1}{3}x^3$, Leading Coefficient = $\frac{1}{3}$, Constant = $3^4$
	\item Degree = 5, Leading Term = $7x^5$, Leading Coefficient = 7, Constant = $-56$
	\item Degree = 7, Leading Term = $-\frac{9}{2}x^7$, Leading Coefficient = $-\frac{9}{2}$, Constant = 2
	\item $\lim_{x \to -\infty} f(x) = \infty \quad \lim_{x \to \infty}f(x) = -\infty$
	\item $\lim_{x \to -\infty} g(x) = -\infty, \quad \lim_{x \to \infty}g(x) = \infty$
	\item $\lim_{x \to -\infty} h(x) = -\infty \quad \lim_{x \to \infty}h(x) =\infty$
	\item $\lim_{x \to -\infty}f(x) = -\infty$ \quad $\lim_{x \to \infty}f(x) = -\infty$
    \item $\lim_{x \to -\infty}g(x) = -\infty$ \quad $\lim_{x \to \infty}g(x) = \infty$
    \item $\lim_{x \to -\infty} f(x) = \infty \quad \lim_{x \to \infty} f(x) = - \infty$
    \item $\lim_{x \to -\infty} g(x) = -\infty \quad \lim_{x \to \infty} g(x) = \infty$
    \item $\lim_{x \to -\infty} h(x) = -\infty \quad \lim_{x \to \infty} h(x) = \infty$
     \item $\lim_{x \to -\infty} j(x) = \infty \quad \lim_{x \to \infty} j(x) = -\infty$
     \item $(-1.92,0), \, (0,0)$
     \item $(0,0), \, (0.83,0)$
     \item $(-0.83,0), \, (0.86,0), \, (1.58,0)$
     \item $(-2.25,0), \, (1.90,0)$
     \item $(-2.48,0), \, (0,0), \, (1.85,0)$
     \item $(-0.42,0), \, (0.79,0)$
     \item $(6.42,0)$
     \item $(-1,0), \, (2,0)$
     \item $\left(-\frac{2}{3},0\right), \, (1,0)$
\end{enumerate}