\chapter{Rational Functions and Their Graphs}

Find the domain, coordinates of any holes, and equations of all asymptotes.
\begin{multicols}{2}
\begin{enumerate}
\setlength\itemsep{10pt}
	\item $f(x) = \frac{2x^2+5x-3}{2x^2-15x+7}$
	\item $g(x) = \frac{3x^3+7x^2-20x}{x^2-x-12}$
	\item $f(x) = \frac{3x}{x+4}$
	\item $g(x) = \frac{x^2+3x+2}{x-1}$
	\item $h(x) = \frac{x^2+3x-4}{x^3-2x^2+x}$
	\item $f(x) = \frac{2x^3-13x^2+6x+45}{x^2-4x-5}$
	\item $g(x) = \frac{5x^2-19x-4}{x^3+2x^2-24x}$
	\item $h(x) = \frac{2x^2-x-3}{8x^2+51x+18}$
	\item $f(x) = \frac{6x^3 - 21x^2 - 51x + 30}{3x^2+7x+2}$
	\item $g(x) = \frac{10x^2-29x-21}{10x^3-33x^2-7x}$
\end{enumerate}	\setcounter{Review}{\value{enumi}}
\end{multicols}
\vspace{0.25in}

State the end behavior of each.
\begin{enumerate}	\setcounter{enumi}{\value{Review}}
	\item $k(x) = \frac{5x^3-7x^2+8}{-3x^3+6x-4}$
	\item $m(x) = \frac{2x-1}{3x^2+7x+1}$
\end{enumerate}

\newpage

\section{Answer Key}

\begin{enumerate}
    \item Domain: $x \neq -\frac{1}{2}, \, 7$; V.A.: $x=7$; Hole @ $\left(-\frac{1}{2},-\frac{7}{13}\right)$; H.A.: $y=1$
    \item Domain: $x \neq -3, \, 4$; V.A.: $x=-3 \, x = 4$; Obl. Asymp: $y = 3x+10$
    \item Domain: $x \neq -4$; V.A.: $x = -4$; H.A.: $y = 3$
    \item Domain: $x \neq 1$; V.A.: $x = 1$; Obl. Asymp: $y = x + 4$
    \item Domain: $x \neq 0, 1$; V.A.: $x = 0$ and $x = 1$; H.A.: $y = 0$ 
    \item Domain: $x \neq -1, 5$; V.A. $x=-1$; Hole @ $\left(5, \frac{13}{3}\right)$; Obl. Asym $y = 2x-5$
    \item Domain: $x \neq -6, 0, 4$; V.A. $x = -6, \, x = 0$; Hole @ $\left(4, \frac{21}{40}\right)$; H.A. $y = 0$
    \item Domain: $x \neq -6, -\frac{3}{8}$; V.A. $x = -6, \, x = -\frac{3}{8}$; H.A. $y = \frac{1}{4}$
    \item Domain: $x \neq -2, \, -\frac{1}{3}$; Hole @ $(-2,-21)$; V.A.: $x = -\frac{1}{3}$; S.A. $y = 2x-\frac{35}{3}$
    \item Domain: $x \neq -\frac{1}{5}, \, 0, \, \frac{7}{2}$; Hole @ $\left(\frac{7}{2}, \frac{82}{259}\right)$; V.A. $x = -\frac{1}{5}$ and $x=0$; H.A. $y=0$
    
%%%%% End Behavior %%%%%%%%%
    \item $\lim_{x \to -\infty} k(x) = \infty = \lim_{x \to \infty} k(x) = -\frac{5}{3}$
    \item $\lim_{x \to -\infty} m(x) = \infty = \lim_{x \to \infty} m(x) = 0$
\end{enumerate}